AXIOMS.md
@@ -296,9 +296,6 @@ Generated from `theories/Substrate/Interface.v` by `scripts/gen-axioms.py`
 | Axiom | `tcp_ptrace_conj_tensorR` | `forall X Y Y' (B : op Y Y') (r : tcp (X * Y)), ocomp (oadj B) B = oid -> tcp_ptrace (tcp_conj (tensoro oid B) r) = tcp_ptrace r` |
 | Axiom | `tcp_ptrace_pswap` | `forall X Y H1 H2 (r : tcp (X * Y)), tcp_ptrace (tcp_conj (@Ubij (X * Y) (Y * X) (fun p => (snd p, fst p)) (fun q => (snd q, fst q)) H1 H2) r) = tcp_ptrace2 r` |
 | Axiom | `tcp_conj_pswap` | `forall X Y H1 H2 (r : tcp X) (s : tcp Y), tcp_conj (@Ubij (X * Y) (Y * X) (fun p => (snd p, fst p)) (fun q => (snd q, fst q)) H1 H2) (tcp_tensor r s) = tcp_tensor s r` |
-| Axiom | `tcp_ptrace2_passoc` | `forall A B C H1 H2 (X : tcp (A * B)) (g : tcp C), tcp_ptrace2 (tcp_conj (@Ubij ((A * B) * C) (A * (B * C)) (fun p => (fst (fst p), (snd (fst p), snd p))) (fun p => ((fst p, fst (snd p)), snd (snd p))) H1 H2) (tcp_tensor X g)) = tcp_tensor (tcp_ptrace2 X) g` |
-| Axiom | `tcp_ptrace_passoc` | `forall A B C H1 H2 (a : tcp A) (Y : tcp (B * C)), tcp_ptrace (tcp_conj (@Ubij (A * (B * C)) ((A * B) * C) (fun p => ((fst p, fst (snd p)), snd (snd p))) (fun p => (fst (fst p), (snd (fst p), snd p))) H1 H2) (tcp_tensor a Y)) = tcp_tensor a (tcp_ptrace Y)` |
-| Axiom | `tcp_ptrace2_passoc_r` | `forall A B C H1 H2 (a : tcp A) (Y : tcp (B * C)), tcp_ptrace2 (tcp_conj (@Ubij (A * (B * C)) ((A * B) * C) (fun p => ((fst p, fst (snd p)), snd (snd p))) (fun p => (fst (fst p), (snd (fst p), snd p))) H1 H2) (tcp_tensor a Y)) = tcp_scale (tcp_trace a) (tcp_ptrace2 Y)` |
 | Axiom | `tcp_tensor_proj` | `forall X Y (v : l2 X) (w : l2 Y), tcp_tensor (tcp_proj v) (tcp_proj w) = tcp_proj (tensorv v w)` |
 | Axiom | `tcp_scale_tensor_l` | `forall X Y (a : R) (r : tcp X) (s : tcp Y), tcp_scale a (tcp_tensor r s) = tcp_tensor (tcp_scale a r) s` |
 | Axiom | `tcp_tensor_add_r` | `forall X Y (r : tcp X) (s t : tcp Y), tcp_tensor r (tcp_add s t) = tcp_add (tcp_tensor r s) (tcp_tensor r t)` |
@@ -320,6 +317,6 @@ Generated from `theories/Substrate/Interface.v` by `scripts/gen-axioms.py`
 | Axiom | `tcp_supp_sum` | `forall X J (F : J -> tcp X), tcp_summable F -> tcp_supp (tcp_sum F) = hSup (fun j => tcp_supp (F j))` |
 | Axiom | `tcp_decompose` | `forall X (r : tcp X), exists (J : Type) (psi : J -> l2 X), tcp_summable (fun j => tcp_proj (psi j)) /\ r = tcp_sum (fun j => tcp_proj (psi j))` |
 
-**Totals: 44 parameters, 131 axioms.**
+**Totals: 44 parameters, 128 axioms.**
 
 <!-- END GENERATED INVENTORY -->
